\documentclass[a4paper,10pt]{article}
\usepackage[T2A]{fontenc}
\usepackage[utf8]{inputenc}
\usepackage{amsmath, amsfonts, amssymb, amsthm, dsfont}
\usepackage{amscd}
\usepackage[russian]{babel}
%\usepackage{pscyr}
\usepackage{cmap}

\textwidth=16.5cm
\hoffset=-2.5cm
\textheight=25.5cm
\voffset=-2.5cm


\righthyphenmin=2
\parindent=0mm
\parskip=3mm

\newcommand{\suml}{\sum\limits}
\newcommand{\intl}{\int\limits}


\DeclareMathOperator*{\esssup}{ess\,sup}
\DeclareMathOperator*{\essinf}{ess\,inf}

%========Библиография=========
\makeatletter
\renewcommand{\@biblabel}[1]{#1.}
\makeatother

\bibliographystyle{utf8gost705u}
%================


\newtheorem{lemma}{Лемма}
\newtheorem{theorem}{Теорема}
\newtheorem*{remark}{Замечание}
%\renewcommand{\theremark}{}
\newtheorem{theoremrus}{Теорема}
\newtheorem{lemmarus}{Лемма}
\newtheorem{statementrus}{Утверждение}
\newtheorem{remarkrus}{Замечание}

\newcommand{\highphantom}{\vphantom{\dfrac{1}{1}}}
\renewcommand{\thesubsubsection}{\arabic{subsubsection}.}

%\renewcommand{\thelemma}{\arabic{lemma}}
%\renewcommand{\proofname}{Доказательство}
\renewcommand{\arraystretch}{2}

\begin{document}
\begin{equation}\label{fib}
  Fib(n)=\frac{\varphi^n - \psi^n}{\sqrt{5}}, \quad
  \varphi = \frac{1+\sqrt{5}}{2},
  \psi = \frac{1-\sqrt{5}}{2}.
\end{equation}
For $n=1, 2$ \eqref{fib} holds. Assume it holds for any $n \le k$. Let's consider the case $n=k+1$. We have to prove that
\begin{equation*}
  Fib(k+1)=\frac{\varphi^{k+1} - \psi^{k+1}}{\sqrt{5}}.
\end{equation*}
Using the recurrence formula and  induction hypothesis we can represent $Fib(k+1)$ as follows:
\begin{multline*}
  Fib(k+1) = Fib(k) + Fib(k-1)=
  \frac{\varphi^{k} - \psi^{k}}{\sqrt{5}} +
  \frac{\varphi^{k-1} - \psi^{k-1}}{\sqrt{5}} = \\
  \frac{1}{2^{k+1}\sqrt{5}}
  \Bigl(
  2(1+\sqrt{5})^k - 2(1-\sqrt{5})^{k} 
  +4(1+\sqrt{5})^{k-1} - 4(1-\sqrt{5})^{k-1} 
  \Bigr)=\\
  \frac{1}{2^{k+1}\sqrt{5}}
  \Bigl(
  (1+\sqrt{5})^{k-1}(2+2\sqrt{5}+4) - (1-\sqrt{5})^{k}((2-2\sqrt{5}+4))
  \Bigr)=\\
  \frac{1}{2^{k+1}\sqrt{5}}
  \Bigl(
  (1+\sqrt{5})^{k-1}(1+\sqrt{5})^2 - (1-\sqrt{5})^{k}(1-\sqrt{5})^2
  \Bigr)=\frac{\varphi^{k+1} - \psi^{k+1}}{\sqrt{5}},
\end{multline*}
thereby showing that our statement holds for $n=k+1$, and formula \eqref{fib} is proved.

It is easy to show that $\Bigl|\frac{\psi^n}{\sqrt{5}}\Bigr|<\frac{1}{2}$. Indeed,
\begin{equation*}
  |\psi| = \frac{\sqrt{5}-1}{2} = \frac{\sqrt{5}}{2} - \frac{1}{2} <
  \frac{\sqrt{9}}{2} - \frac{1}{2} = 1,
\end{equation*}
so $\Bigl|\frac{\psi^n}{\sqrt{5}}\Bigr| < \frac{1}{\sqrt{5}} < \frac{1}{2}$.
\end{document}
